coq/Puiseux_series.v
@@ -1,0 +1,298 @@
+(* $Id: Puiseux_series.v,v 1.1 2013-06-24 01:37:46 deraugla Exp $ *)
+
+Require Import Utf8.
+Require Import QArith.
+
+Require Import Field.
+Require Import Series.
+
+Set Implicit Arguments.
+
+Record term α := { coeff : α; power : Q }.
+
+Definition den_divides_comden comden p :=
+  (' Qden p | (Zpos comden * Qnum p))%Z.
+
+Definition pow_den_div_com_den α comden (t : term α) :=
+  den_divides_comden comden (power t).
+
+Record puiseux_series α :=
+  { ps_terms : series (term α);
+    ps_comden : positive;
+    ps_prop : series_forall (pow_den_div_com_den ps_comden) ps_terms }.
+
+(* [series_head] skip the possible terms with null coefficients and return
+   the sub-series of the initial series whose coefficient of the first term
+   is not null. E.g.: applied to
+       0+0x³+5x⁵+0x⁷+3x⁸+...
+   would return
+       5x⁵+0x⁷+3x⁸+... *)
+Definition series_head : ∀ α, (α → bool) → series (term α) → series (term α).
+Proof. Admitted.
+
+Definition valuation α fld (ps : puiseux_series α) :=
+  match series_head (is_zero fld) (ps_terms ps) with
+  | Term mx _ => Some (power mx)
+  | End => None
+  end.
+
+Definition valuation_coeff α fld (ps : puiseux_series α) :=
+  match series_head (is_zero fld) (ps_terms ps) with
+  | Term mx _ => coeff mx
+  | End => zero fld
+  end.
+
+(* ps_add *)
+
+CoFixpoint ps_add_loop α (add_coeff : α → α → α) ms₁ ms₂ :=
+  match ms₁ with
+  | Term c₁ s₁ =>
+      match ms₂ with
+      | Term c₂ s₂ =>
+          match Qcompare (power c₁) (power c₂) with
+          | Eq =>
+              let c := add_coeff (coeff c₁) (coeff c₂) in
+              let m := {| coeff := c; power := power c₁ |} in
+              Term m (ps_add_loop add_coeff s₁ s₂)
+          | Lt =>
+              Term c₁ (ps_add_loop add_coeff s₁ ms₂)
+          | Gt =>
+              Term c₂ (ps_add_loop add_coeff ms₁ s₂)
+          end
+      | End => ms₁
+      end
+  | End => ms₂
+  end.
+
+Definition Plcm a b := Z.to_pos (Z.lcm (Zpos a) (Zpos b)).
+
+Lemma Zlcm_pos : ∀ a b, (0 < Z.lcm (Zpos a) (Zpos b))%Z.
+Proof.
+intros a b.
+unfold Z.lcm.
+rewrite Z.abs_mul.
+remember (Z.abs (' a)) as x; simpl in Heqx; subst x.
+apply Z.mul_pos_pos; [ apply Pos2Z.is_pos | idtac ].
+apply Z.abs_pos; simpl.
+intros H.
+apply Z.div_small_iff in H.
+ destruct H as [H| H].
+  destruct H as (Hb, Hbg).
+  pose proof (Pos.gcd_divide_r a b) as H.
+  destruct H as (z, H).
+  rewrite H in Hbg at 1.
+  rewrite Pos2Z.inj_mul in Hbg.
+  remember (Pos.gcd a b) as x.
+  remember (' z * ' x)%Z as y.
+  replace (' x)%Z with (1 * ' x)%Z in Hbg by reflexivity; subst y.
+  apply Zmult_lt_reg_r in Hbg; [ idtac | apply Pos2Z.is_pos ].
+  apply Zlt_le_succ in Hbg.
+  revert Hbg.
+  apply Zlt_not_le, Z.lt_pred_lt_succ; simpl.
+  apply Pos2Z.is_pos.
+
+  destruct H as (Hg, Hb).
+  revert Hb.
+  apply Zlt_not_le, Pos2Z.is_pos.
+
+ pose proof (Pos2Z.is_pos (Pos.gcd a b)) as HH.
+ intros HHH.
+ rewrite HHH in HH; apply Zlt_irrefl in HH; assumption.
+Qed.
+
+Lemma div_div_lcm : ∀ α a b (t : term α),
+  pow_den_div_com_den a t
+  → pow_den_div_com_den (Plcm a b) t.
+Proof.
+intros α a b t H.
+unfold pow_den_div_com_den in H |- *.
+unfold den_divides_comden in H |- *.
+destruct H as (k, H).
+unfold Z.divide.
+unfold Plcm.
+pose proof (Z.divide_lcm_l (' a) (' b)) as Hl.
+destruct Hl as (k₁, Hl).
+rewrite Hl.
+destruct k₁.
+ pose proof (Zlcm_pos a b)%Z as HH.
+ rewrite Hl in HH; apply Zlt_irrefl in HH; contradiction.
+
+ rewrite Z2Pos.inj_mul; try apply Pos2Z.is_pos.
+ do 2 rewrite Pos2Z.id.
+ rewrite Pos2Z.inj_mul.
+ rewrite <- Zmult_assoc, H, Zmult_assoc.
+ exists (' p * k)%Z; reflexivity.
+
+ pose proof (Zlcm_pos a b)%Z as HH.
+ rewrite Hl in HH.
+ simpl in HH.
+ apply Zlt_not_le in HH.
+ exfalso; apply HH.
+ apply Zlt_le_weak, Zlt_neg_0.
+Qed.
+
+Lemma Pos_divide_lcm_l : ∀ a b, (a | Plcm a b)%positive.
+Proof.
+intros a b.
+unfold Plcm.
+pose proof (Zlcm_pos a b)%Z as H.
+unfold Z.lcm.
+rewrite Z.abs_mul.
+rewrite Z2Pos.inj_mul.
+ remember (' b / Z.gcd (' a) (' b))%Z as x.
+ simpl.
+ rewrite Pmult_comm.
+ exists (Z.to_pos (Z.abs x)); reflexivity.
+
+ simpl.
+ apply Pos2Z.is_pos.
+
+ unfold Z.lcm in H.
+ rewrite Z.abs_mul in H.
+ remember (' b / Z.gcd (' a) (' b))%Z as x.
+ apply Z.lt_0_mul in H.
+ destruct H as [H| H].
+  destruct H; assumption.
+
+  destruct H as (_, H).
+  apply Zlt_not_le in H.
+  exfalso; apply H.
+  apply Z.abs_nonneg.
+Qed.
+
+Lemma Pos_divide_lcm_r : ∀ a b, (b | Plcm a b)%positive.
+Proof.
+intros a b.
+unfold Plcm.
+rewrite Z.lcm_comm.
+apply Pos_divide_lcm_l.
+Qed.
+
+Lemma series_forall_div_mul : ∀ α (s : series (term α)) cd x,
+  series_forall (pow_den_div_com_den cd) s
+  → series_forall (pow_den_div_com_den (cd * x)) s.
+Proof.
+cofix IHs.
+intros α s cd x H.
+destruct s as [t s| ]; [ idtac | constructor; reflexivity ].
+eapply TermAndFurther; [ reflexivity | idtac | idtac ].
+ apply series_forall_inv in H.
+ destruct H as (H, _).
+ unfold pow_den_div_com_den in H |- *.
+ destruct H as (k₁, H).
+ rewrite Pmult_comm.
+ unfold den_divides_comden.
+ exists (Zpos x * k₁)%Z.
+ rewrite Pos2Z.inj_mul.
+ rewrite <- Zmult_assoc, H, Zmult_assoc.
+ reflexivity.
+
+ apply series_forall_inv in H.
+ destruct H as (_, H).
+ eapply IHs; eassumption.
+Qed.
+
+Lemma series_forall_add : ∀ α (add_coeff : α → α → α) s₁ s₂ cd₁ cd₂,
+  series_forall (pow_den_div_com_den cd₁) s₁
+  → series_forall (pow_den_div_com_den cd₂) s₂
+    → series_forall (pow_den_div_com_den (Plcm cd₁ cd₂))
+        (ps_add_loop add_coeff s₁ s₂).
+Proof.
+cofix IHs.
+intros α add_coeff s₁ s₂ cd₁ cd₂ Hps₁ Hps₂.
+rewrite series_eta; simpl.
+destruct s₁.
+ rename t into t₁.
+ destruct s₂.
+  rename t into t₂.
+  remember (power t₁ ?= power t₂) as c.
+  symmetry in Heqc.
+  destruct c.
+   apply Qeq_alt in Heqc.
+   eapply TermAndFurther; [ reflexivity | idtac | idtac ].
+    apply series_forall_inv in Hps₁.
+    destruct Hps₁ as (Hpd₁, Hsf₁).
+    unfold pow_den_div_com_den in Hpd₁ |- *; simpl.
+    destruct Hpd₁ as (k₁, Hpd₁).
+    unfold den_divides_comden.
+    unfold Z.divide.
+    exists (Zpos (Plcm cd₁ cd₂) / Zpos cd₁ * k₁)%Z.
+    rewrite <- Zmult_assoc, <- Hpd₁.
+    rewrite Zmult_assoc.
+    f_equal.
+    rewrite Zmult_comm.
+    rewrite <- Z.divide_div_mul_exact.
+     rewrite Zmult_comm.
+     rewrite Z.div_mul; [ reflexivity | intros H; discriminate H ].
+
+     pose proof (Pos2Z.is_pos cd₁) as H.
+     intros HH; rewrite HH in H; apply Zlt_irrefl in H; assumption.
+
+     unfold Plcm.
+     rewrite Z2Pos.id; [ apply Z.divide_lcm_l | apply Zlcm_pos ].
+
+    apply IHs; eapply series_forall_inv; eassumption.
+
+   eapply TermAndFurther; [ reflexivity | idtac | idtac ].
+    apply series_forall_inv in Hps₁.
+    destruct Hps₁ as (Hpd₁, Hps₁).
+    apply div_div_lcm; assumption.
+
+    apply IHs; [ eapply series_forall_inv; eassumption | assumption ].
+
+   eapply TermAndFurther; [ reflexivity | idtac | idtac ].
+    apply series_forall_inv in Hps₂.
+    destruct Hps₂ as (Hpd₂, Hps₂).
+    unfold Plcm.
+    rewrite Z.lcm_comm.
+    apply div_div_lcm; assumption.
+
+    apply IHs; [ assumption | idtac ].
+    apply series_forall_inv in Hps₂.
+    destruct Hps₂; assumption.
+
+  eapply TermAndFurther; [ reflexivity | idtac | idtac ].
+   apply series_forall_inv in Hps₁.
+   destruct Hps₁ as (Hpd₁, Hsf₁).
+   apply div_div_lcm; assumption.
+
+   pose proof (Pos_divide_lcm_l cd₁ cd₂) as H.
+   destruct H as (z, H).
+   rewrite H, Pos.mul_comm.
+   apply series_forall_div_mul.
+   apply series_forall_inv in Hps₁.
+   destruct Hps₁; assumption.
+
+ destruct s₂.
+  rename t into t₂.
+  eapply TermAndFurther; [ reflexivity | idtac | idtac ].
+   apply series_forall_inv in Hps₂.
+   destruct Hps₂ as (Hpd₂, Hsf₂).
+   unfold pow_den_div_com_den in Hpd₂ |- *.
+   unfold Plcm.
+   rewrite Z.lcm_comm.
+   apply div_div_lcm; assumption.
+
+   pose proof (Pos_divide_lcm_r cd₁ cd₂) as H.
+   destruct H as (z, H).
+   rewrite H, Pos.mul_comm.
+   apply series_forall_div_mul.
+   apply series_forall_inv in Hps₂.
+   destruct Hps₂; assumption.
+
+  constructor; reflexivity.
+Qed.
+
+Theorem ps_prop_add : ∀ α (add_coeff : α → α → α) ps₁ ps₂,
+  series_forall
+    (pow_den_div_com_den (Plcm (ps_comden ps₁) (ps_comden ps₂)))
+    (ps_add_loop add_coeff (ps_terms ps₁) (ps_terms ps₂)).
+Proof.
+intros α add_coeff ps₁ ps₂.
+apply series_forall_add; [ apply (ps_prop ps₁) | apply (ps_prop ps₂) ].
+Qed.
+
+Definition ps_add α (add_coeff : α → α → α) (ps₁ ps₂ : puiseux_series α) :=
+  {| ps_terms := ps_add_loop add_coeff (ps_terms ps₁) (ps_terms ps₂);
+     ps_comden := Plcm (ps_comden ps₁) (ps_comden ps₂);
+     ps_prop := ps_prop_add add_coeff ps₁ ps₂ |}.
